Utils.fst
@@ -1,0 +1,13 @@
+module Utils 
+
+(* imported modules *)
+open Structs
+(* ---------------- *)
+
+
+let print_pyObj p =
+  match p with
+  | INT i -> Printf.sprintf "INT: %d" i
+  | STRING s -> Printf.sprintf "STRING: %s" s
+  | NONE -> Printf.sprintf "NONE"
+  | ERR s -> Printf.sprintf "ERR: %s" s
