VM.fsti
@@ -5,10 +5,11 @@ open Structs
 (* ---------------- *)
 
 (* Creates a new frame and push it to the frame stack *)
-val makeFrame: vm -> codeObj -> (vm * frameObj)
+val makeFrame: vm -> codeObj ->  (vm * frameObj)
 
 (* Run Frame and then pop it from call stack when you done *)
-val runFrame: vm -> frameObj -> All.ML (vm * pyObj)
+(* val runFrame: vm -> frameObj -> All.ML (vm * pyObj) *)
+val runFrame: vm -> frameObj -> All.ML pyObj
 
 (* Takes in code object and execute it *)
 val runCode: codeObj -> All.ML pyObj
